## Exercise S7: #3
```
let cond c then_e else_e = 
    if c then then_e else else_e
```
## Exercise S7: #4
```
sum (take 3 (squares_from 1))
sum (take 3 (v*v :: squares_from (v+1)))
    where v = 1
sum (v*v :: take (3-1) (squares_from (v+1)))
    where v = 1
(v+v) + sum (take (3-1) (squares_from (v+1)))
    where v = 1
(1*1) + sum (take (3-1) (square_from (1+1)))
1 + sum (take (3-1) (squares_from (1+1)))
1 + sum (take 2 (squares_from (1+1)))
1+ sum (take 2 (v*v :: squares_from (v+1)))
    where v = 1+1
.
.
.
```